src/HOL/Lambda/ListApplication.thy
@@ -6,9 +6,157 @@
 Application of a term to a list of terms
 *)
 
-ListApplication = Lambda +
+theory ListApplication = Lambda:
 
-syntax "$$" :: dB => dB list => dB (infixl 150)
-translations "t $$ ts" == "foldl op$ t ts"
+syntax
+  "_list_application" :: "dB => dB list => dB"   (infixl "$$" 150)
+translations
+  "t $$ ts" == "foldl (op $) t ts"
+
+
+lemma apps_eq_tail_conv [iff]: "(r $$ ts = s $$ ts) = (r = s)"
+  apply (induct_tac ts rule: rev_induct)
+   apply auto
+  done
+
+lemma Var_eq_apps_conv [rulify, iff]:
+    "\<forall>s. (Var m = s $$ ss) = (Var m = s \<and> ss = [])"
+  apply (induct_tac ss)
+   apply auto
+  done
+
+lemma Var_apps_eq_Var_apps_conv [rulify, iff]:
+    "\<forall>ss. (Var m $$ rs = Var n $$ ss) = (m = n \<and> rs = ss)"
+  apply (induct_tac rs rule: rev_induct)
+   apply simp
+   apply blast
+  apply (rule allI)
+  apply (induct_tac ss rule: rev_induct)
+   apply auto
+  done
+
+lemma App_eq_foldl_conv:
+  "(r $ s = t $$ ts) =
+    (if ts = [] then r $ s = t
+    else (\<exists>ss. ts = ss @ [s] \<and> r = t $$ ss))"
+  apply (rule_tac xs = ts in rev_exhaust)
+   apply auto
+  done
+
+lemma Abs_eq_apps_conv [iff]:
+    "(Abs r = s $$ ss) = (Abs r = s \<and> ss = [])"
+  apply (induct_tac ss rule: rev_induct)
+   apply auto
+  done
+
+lemma apps_eq_Abs_conv [iff]: "(s $$ ss = Abs r) = (s = Abs r \<and> ss = [])"
+  apply (induct_tac ss rule: rev_induct)
+   apply auto
+  done
+
+lemma Abs_apps_eq_Abs_apps_conv [iff]:
+    "\<forall>ss. (Abs r $$ rs = Abs s $$ ss) = (r = s \<and> rs = ss)"
+  apply (induct_tac rs rule: rev_induct)
+   apply simp
+   apply blast
+  apply (rule allI)
+  apply (induct_tac ss rule: rev_induct)
+   apply auto
+  done
+
+lemma Abs_App_neq_Var_apps [iff]:
+    "\<forall>s t. Abs s $ t ~= Var n $$ ss"
+  apply (induct_tac ss rule: rev_induct)
+   apply auto
+  done
+
+lemma Var_apps_neq_Abs_apps [rulify, iff]:
+    "\<forall>ts. Var n $$ ts ~= Abs r $$ ss"
+  apply (induct_tac ss rule: rev_induct)
+   apply simp
+  apply (rule allI)
+  apply (induct_tac ts rule: rev_induct)
+   apply auto
+  done
+
+lemma ex_head_tail:
+  "\<exists>ts h. t = h $$ ts \<and> ((\<exists>n. h = Var n) \<or> (\<exists>u. h = Abs u))"
+  apply (induct_tac t)
+    apply (rule_tac x = "[]" in exI)
+    apply simp
+   apply clarify
+   apply (rename_tac ts1 ts2 h1 h2)
+   apply (rule_tac x = "ts1 @ [h2 $$ ts2]" in exI)
+   apply simp
+  apply simp
+  done
+
+lemma size_apps [simp]:
+  "size (r $$ rs) = size r + foldl (op +) 0 (map size rs) + length rs"
+  apply (induct_tac rs rule: rev_induct)
+   apply auto
+  done
+
+lemma lem0: "[| (0::nat) < k; m <= n |] ==> m < n + k"
+  apply simp
+  done
+
+text {* A customized induction schema for @{text "$$"} *}
+
+lemma lem [rulify]:
+  "[| !!n ts. \<forall>t \<in> set ts. P t ==> P (Var n $$ ts);
+      !!u ts. [| P u; \<forall>t \<in> set ts. P t |] ==> P (Abs u $$ ts)
+  |] ==> \<forall>t. size t = n --> P t"
+proof -
+  case antecedent
+  show ?thesis
+   apply (induct_tac n rule: less_induct)
+   apply (rule allI)
+   apply (cut_tac t = t in ex_head_tail)
+   apply clarify
+   apply (erule disjE)
+    apply clarify
+    apply (rule prems)
+    apply clarify
+    apply (erule allE, erule impE)
+      prefer 2
+      apply (erule allE, erule mp, rule refl)
+     apply simp
+     apply (rule lem0)
+      apply force
+     apply (rule elem_le_sum)
+     apply force
+    apply clarify
+    apply (rule prems)
+     apply (erule allE, erule impE)
+      prefer 2
+      apply (erule allE, erule mp, rule refl)
+     apply simp
+    apply clarify
+    apply (erule allE, erule impE)
+     prefer 2
+     apply (erule allE, erule mp, rule refl)
+    apply simp
+    apply (rule le_imp_less_Suc)
+    apply (rule trans_le_add1)
+    apply (rule trans_le_add2)
+    apply (rule elem_le_sum)
+    apply force
+    done
+qed
+
+lemma Apps_dB_induct:
+  "[| !!n ts. \<forall>t \<in> set ts. P t ==> P (Var n $$ ts);
+      !!u ts. [| P u; \<forall>t \<in> set ts. P t |] ==> P (Abs u $$ ts)
+  |] ==> P t"
+proof -
+  case antecedent
+  show ?thesis
+    apply (rule_tac t = t in lem)
+      prefer 3
+      apply (rule refl)
+     apply (assumption | rule prems)+
+    done
+qed
 
 end
