src/HOL/Lambda/ListOrder.thy
@@ -6,11 +6,111 @@
 Lifting an order to lists of elements, relating exactly one element
 *)
 
-ListOrder = Acc +
+theory ListOrder = Acc:
 
 constdefs
- step1 :: "('a * 'a)set => ('a list * 'a list)set"
-"step1 r ==
-   {(ys,xs). ? us z z' vs. xs = us@z#vs & (z',z) : r & ys = us@z'#vs}"
+  step1 :: "('a \<times> 'a) set => ('a list \<times> 'a list) set"
+  "step1 r ==
+    {(ys, xs). \<exists>us z z' vs. xs = us @ z # vs \<and> (z', z) \<in> r \<and> ys = us @ z' # vs}"
+
+
+lemma step1_converse [simp]: "step1 (r^-1) = (step1 r)^-1"
+  apply (unfold step1_def)
+  apply blast
+  done
+
+lemma in_step1_converse [iff]: "(p \<in> step1 (r^-1)) = (p \<in> (step1 r)^-1)"
+  apply auto
+  done
+
+lemma not_Nil_step1 [iff]: "([], xs) \<notin> step1 r"
+  apply (unfold step1_def)
+  apply blast
+  done
+
+lemma not_step1_Nil [iff]: "(xs, []) \<notin> step1 r"
+  apply (unfold step1_def)
+  apply blast
+  done
+
+lemma Cons_step1_Cons [iff]:
+  "((y # ys, x # xs) \<in> step1 r) = ((y, x) \<in> r \<and> xs = ys \<or> x = y \<and> (ys, xs) \<in> step1 r)"
+  apply (unfold step1_def)
+  apply simp
+  apply (rule iffI)
+   apply (erule exE)
+   apply (rename_tac ts)
+   apply (case_tac ts)
+    apply force
+   apply force
+  apply (erule disjE)
+   apply blast
+  apply (blast intro: Cons_eq_appendI)
+  done
+
+lemma append_step1I:
+  "(ys, xs) \<in> step1 r \<and> vs = us \<or> ys = xs \<and> (vs, us) \<in> step1 r
+    ==> (ys @ vs, xs @ us) : step1 r"
+  apply (unfold step1_def)
+  apply auto
+   apply blast
+  apply (blast intro: append_eq_appendI)
+  done
+
+lemma Cons_step1E [rulify_prems, elim!]:
+  "[| (ys, x # xs) \<in> step1 r;
+      \<forall>y. ys = y # xs --> (y, x) \<in> r --> R;
+      \<forall>zs. ys = x # zs --> (zs, xs) : step1 r --> R
+   |] ==> R"
+  apply (case_tac ys)
+   apply (simp add: step1_def)
+  apply blast
+  done
+
+lemma Snoc_step1_SnocD:
+  "(ys @ [y], xs @ [x]) \<in> step1 r
+    ==> ((ys, xs) \<in> step1 r \<and> y = x \<or> ys = xs \<and> (y, x) \<in> r)"
+  apply (unfold step1_def)
+  apply simp
+  apply (clarify del: disjCI)
+  apply (rename_tac vs)
+  apply (rule_tac xs = vs in rev_exhaust)
+   apply force
+  apply simp
+  apply blast
+  done
+
+lemma Cons_acc_step1I [rulify, intro!]:
+    "x \<in> acc r ==> \<forall>xs. xs \<in> acc (step1 r) --> x # xs \<in> acc (step1 r)"
+  apply (erule acc_induct)
+  apply (erule thin_rl)
+  apply clarify
+  apply (erule acc_induct)
+  apply (rule accI)
+  apply blast
+  done
+
+lemma lists_accD: "xs \<in> lists (acc r) ==> xs \<in> acc (step1 r)"
+  apply (erule lists.induct)
+   apply (rule accI)
+   apply simp
+  apply (rule accI)
+  apply (fast dest: acc_downward)
+  done
+
+lemma ex_step1I: "[| x \<in> set xs; (y, x) \<in> r |]
+    ==> \<exists>ys. (ys, xs) \<in> step1 r \<and> y \<in> set ys"
+  apply (unfold step1_def)
+  apply (drule in_set_conv_decomp [THEN iffD1])
+  apply force
+  done
+
+lemma lists_accI: "xs \<in> acc (step1 r) ==> xs \<in> lists (acc r)"
+  apply (erule acc_induct)
+  apply clarify
+  apply (rule accI)
+  apply (drule ex_step1I, assumption)
+  apply blast
+  done
 
 end
